Makefile
@@ -197,6 +197,7 @@ print-assumptions: category-theory
 	  echo 'Require Import Category.Structure.Monoidal.Hypergraph.Spider.'; \
 	  echo 'Require Import Category.Instance.ZX.'; \
 	  echo 'Require Import Category.Theory.Lambek.'; \
+	  echo 'Require Import Category.Instance.Grp.'; \
 	  echo 'Require Import Category.Adjunction.GAFT.'; \
 	  echo 'Require Import Category.Monad.Monadicity.Beck.'; \
 	  echo 'Require Import Category.Construction.Grothendieck.RoundTrip.'; \
@@ -214,6 +215,9 @@ print-assumptions: category-theory
 	  echo 'Print Assumptions ZX_Cat.'; \
 	  echo 'Print Assumptions Hypergraph_CompactClosed.'; \
 	  echo 'Print Assumptions lambek.'; \
+	  echo 'Print Assumptions Grp.'; \
+	  echo 'Print Assumptions Grp_Forget.'; \
+	  echo 'Print Assumptions Grp_Zero.'; \
 	  echo 'Print Assumptions GAFT.'; \
 	  echo 'Print Assumptions beck_monadicity.'; \
 	  echo 'Print Assumptions monadic_creates.'; \
